First-cut proof of correctness of iterative algorithm.

src/dafny/smart/incAlgoV3.dfy
@@ -116,30 +116,211 @@ module IncAlgoV3 {
 
         decreases h
     {
-    if h == 1 then
-        var r := computeRootPathDiff([k as bit], valOnLeftAt, seed);
-        assert(valOnLeftAt ==  [valOnLeftAt[0]]);
-        (r, if k == 0 then [seed] else [valOnLeftAt[h - 1]]) 
-    else 
-        if k % 2 == 0 then
-            var r := computeRootPathDiffAndLeftSiblingsUpv4(
+        if h == 1 then
+            var r := computeRootPathDiff([k as bit], valOnLeftAt, seed);
+            assert(valOnLeftAt ==  [valOnLeftAt[0]]);
+            (r, if k == 0 then [seed] else [valOnLeftAt[h - 1]]) 
+        else 
+            if k % 2 == 0 then
+                var r := computeRootPathDiffAndLeftSiblingsUpv4(
+                            h - 1,
+                            k / 2,
+                            valOnLeftAt[..h - 1],   
+                            diff(seed, 0) );
+                (r.0, valOnLeftAt[.. h - 1] + [seed])
+            else      
+                var r :=  computeRootPathDiffAndLeftSiblingsUpv4(
                         h - 1,
                         k / 2,
-                        valOnLeftAt[..h - 1],   
-                        diff(seed, 0) );
-                    (r.0, valOnLeftAt[.. h - 1] + [seed])
-        else      
-            var r :=  computeRootPathDiffAndLeftSiblingsUpv4(
-                    h - 1,
-                    k / 2,
-                    valOnLeftAt[..h - 1],  
-                    diff(valOnLeftAt[h - 1], seed));
-                    /*  The last value [valOnLeftAt[|valOnLeftAt| - 1]] is not used on 
-                        the next path as it is not a leftSibling of a node of next path.
-                        at this level. As a consequence we can use any value to append to
-                        the second component of the result .1. We just use the old value 
-                        [valOnLeftAt[|valOnLeftAt| - 1] as it will enable us to "modify" 
-                        in-place a unique array in the imperative version. */
-                    (r.0, r.1 + [valOnLeftAt[h - 1]])
+                        valOnLeftAt[..h - 1],  
+                        diff(valOnLeftAt[h - 1], seed));
+                        /*  The last value [valOnLeftAt[|valOnLeftAt| - 1]] is not used on 
+                            the next path as it is not a leftSibling of a node of next path.
+                            at this level. As a consequence we can use any value to append to
+                            the second component of the result .1. We just use the old value 
+                            [valOnLeftAt[|valOnLeftAt| - 1] as it will enable us to "modify" 
+                            in-place a unique array in the imperative version. */
+                (r.0, r.1 + [valOnLeftAt[h - 1]])
+    }
+
+    /**
+     *  For path of size >= 2, computeRootPathDiffAndLeftSiblingsUp and computeRootPathDiffUp
+     *  yield the same result.
+     */
+    lemma  computeRootAndSiblingsV4IsCorrect(h : nat,
+        k : nat,
+        valOnLeftAt : seq<int>, seed: int)
+        requires 1 <= h == |valOnLeftAt|
+        requires k < power2(h)
+
+        ensures  computeRootPathDiffAndLeftSiblingsUpv4(h, k, valOnLeftAt, seed) == 
+            (computeRootPathDiffUp(natToBitList(k, h), valOnLeftAt, seed),
+            computeLeftSiblingOnNextPath(natToBitList(k, h), computeAllPathDiffUp(natToBitList(k, h), valOnLeftAt, seed), valOnLeftAt)
+            )
+
+    {   
+        /*
+         *  V4 computes same as V3, same as V2 and V2 is correct.
+         */
+        calc == {
+            computeRootPathDiffAndLeftSiblingsUpv4(h, k, valOnLeftAt, seed);
+            computeRootPathDiffAndLeftSiblingsUpv3(natToBitList(k, h), h, k, valOnLeftAt, seed);
+            computeRootPathDiffAndLeftSiblingsUpv2(natToBitList(k, h), valOnLeftAt, seed);
+            {
+                computeRootAndSiblingsv2IsCorrect(natToBitList(k, h),  valOnLeftAt, seed);
+            }
+            (computeRootPathDiffUp(natToBitList(k, h), valOnLeftAt, seed),
+            computeLeftSiblingOnNextPath(natToBitList(k, h), 
+                computeAllPathDiffUp(natToBitList(k, h), valOnLeftAt, seed), valOnLeftAt));
+        }   
+    }
+
+   /**
+     *  Use the natural value of a path and height (supposedly of the tree) 
+     *  to compute the results. Stop at h == 0 instead of h == 1. 
+     */
+    function method computeRootPathDiffAndLeftSiblingsUpv4b(
+        h : nat,
+        k : nat,
+        valOnLeftAt : seq<int>, seed: int) : (int, seq<int>)
+        requires 0 <= h == |valOnLeftAt|
+        // requires h > 0 ==> k < power2(h)
+        requires k < power2(h)
+
+        decreases h
+    {
+        if h == 0 then
+            (seed, [])
+        else 
+            if k % 2 == 0 then
+                var r := computeRootPathDiffAndLeftSiblingsUpv4b(
+                            h - 1,
+                            k / 2,
+                            valOnLeftAt[..h - 1],   
+                            diff(seed, 0) );
+                (r.0, valOnLeftAt[..h - 1] + [seed])
+            else      
+                var r :=  computeRootPathDiffAndLeftSiblingsUpv4b(
+                        h - 1,
+                        k / 2,
+                        valOnLeftAt[..h - 1],  
+                        diff(valOnLeftAt[h - 1], seed));
+                        /*  The last value [valOnLeftAt[|valOnLeftAt| - 1]] is not used on 
+                            the next path as it is not a leftSibling of a node of next path.
+                            at this level. As a consequence we can use any value to append to
+                            the second component of the result .1. We just use the old value 
+                            [valOnLeftAt[|valOnLeftAt| - 1] as it will enable us to "modify" 
+                            in-place a unique array in the imperative version. */
+                (r.0, r.1 + [valOnLeftAt[h - 1]])
+    }
+
+    lemma  computeRootAndSiblingsV4bIsCorrect(h : nat,
+        k : nat,
+        valOnLeftAt : seq<int>, seed: int)
+        requires 1 <= h == |valOnLeftAt|
+        requires k < power2(h)
+
+        ensures  computeRootPathDiffAndLeftSiblingsUpv4b(h, k, valOnLeftAt, seed) == 
+           computeRootPathDiffAndLeftSiblingsUpv4(h, k, valOnLeftAt, seed)
+    {
+        if ( h >= 2 ) {
+            //  if h >= 2 they compute exactly the same. Thanks Dafny
+        } else {
+            //  The only interesting case is h == 1
+            //  If h == 1 then k == 0 or k == 1. We show that v4b computes same as v4
+            //  by unfolding the computation.
+            if (k % 2 == 0) {
+                var r := computeRootPathDiffAndLeftSiblingsUpv4b(0, 0, [], diff(seed, 0));
+
+                calc {
+                    computeRootPathDiffAndLeftSiblingsUpv4b(h, k, valOnLeftAt, seed);
+                    (r.0, valOnLeftAt[..h - 1] + [seed]);    
+                    calc {
+                        [] + [seed];
+                        [seed];
+                    }
+                    (r.0, [seed]);
+                    calc {
+                        r.0;
+                        diff(seed, 0);
+                    }
+                    (diff(seed, 0), [seed]);
+                    (computeRootPathDiff([0], valOnLeftAt, seed), [seed]);
+                }
+                //  Thanks Dafny
+            } else {
+                //   k % 2 == 1 and k == 1
+                var r := computeRootPathDiffAndLeftSiblingsUpv4b(0, 0, [], diff(valOnLeftAt[0], seed));
+                calc {
+                    computeRootPathDiffAndLeftSiblingsUpv4b(h, k, valOnLeftAt, seed);
+                    (r.0, r.1 + [valOnLeftAt[h - 1]]);
+                    calc {
+                        r.1 + [valOnLeftAt[h - 1]];
+                        [] + [valOnLeftAt[h - 1]];
+                        [valOnLeftAt[h - 1]];
+                    }
+                    (r.0, [valOnLeftAt[h - 1]]);
+                    (diff(valOnLeftAt[h - 1], seed), [valOnLeftAt[h - 1]]);
+                    (computeRootPathDiff([1], valOnLeftAt, seed),  [valOnLeftAt[h - 1]]);
+                }
+            }
+        }
+    }
+
+    /**
+     *  Tail recursive version of algorithm.
+     */
+    function method computeRootPathDiffAndLeftSiblingsUpv4c(
+        h : nat,
+        k : nat,
+        valOnLeftAt : seq<int>, 
+        seed: int,
+        newLeft : seq<int>) : (int, seq<int>)
+        requires 0 <= h == |valOnLeftAt|
+        // requires h > 0 ==> k < power2(h)
+        // requires |valOnLeftAt| + |newLeft| == h 
+        requires k < power2(h)
+
+
+        decreases h
+    {
+        if h == 0 then
+            (seed, newLeft)
+        else 
+            if k % 2 == 0 then
+                computeRootPathDiffAndLeftSiblingsUpv4c(
+                            h - 1,
+                            k / 2,
+                            valOnLeftAt[..h - 1],   
+                            diff(seed, 0),
+                            [seed] + newLeft)
+            else      
+                computeRootPathDiffAndLeftSiblingsUpv4c(
+                        h - 1,
+                        k / 2,
+                        valOnLeftAt[..h - 1],  
+                        diff(valOnLeftAt[h - 1], seed),
+                        [valOnLeftAt[h - 1]] + newLeft)
+                        /*  The last value [valOnLeftAt[|valOnLeftAt| - 1]] is not used on 
+                            the next path as it is not a leftSibling of a node of next path.
+                            at this level. As a consequence we can use any value to append to
+                            the second component of the result .1. We just use the old value 
+                            [valOnLeftAt[|valOnLeftAt| - 1] as it will enable us to "modify" 
+                            in-place a unique array in the imperative version. */
+    }
+
+     lemma  {:induction h} computeRootAndSiblingsV4cIsCorrect(h : nat,
+        k : nat,
+        valOnLeftAt : seq<int>, seed: int,  newLeft : seq<int>)
+        requires 1 <= h == |valOnLeftAt|
+        requires k < power2(h)
+        requires |valOnLeftAt| + |newLeft| == h - 1
+
+        ensures |computeRootPathDiffAndLeftSiblingsUpv4c(h, k, valOnLeftAt, seed, []).1| == h
+
+        ensures  computeRootPathDiffAndLeftSiblingsUpv4b(h, k, valOnLeftAt, seed) == 
+           computeRootPathDiffAndLeftSiblingsUpv4c(h, k, valOnLeftAt, seed, [])
+    {   
+        //  Thanks Dafny
     }
  }
