src/dafny/smart/incAlgoV5.dfy
@@ -1,0 +1,155 @@
+/*
+ * Copyright 2020 ConsenSys AG.
+ *
+ * Licensed under the Apache License, Version 2.0 (the "License"); you may 
+ * not use this file except in compliance with the License. You may obtain 
+ * a copy of the License at http://www.apache.org/licenses/LICENSE-2.0
+ *
+ * Unless required by applicable law or agreed to in writing, software dis-
+ * tributed under the License is distributed on an "AS IS" BASIS, WITHOUT 
+ * WARRANTIES OR CONDITIONS OF ANY KIND, either express or implied. See the 
+ * License for the specific language governing permissions and limitations 
+ * under the License.
+ */
+ 
+include "DiffTree.dfy"
+
+include "IncAlgoV3.dfy"
+include "CompleteTrees.dfy"
+include "ComputeRootPath.dfy"
+include "GenericComputation.dfy"
+include "Helpers.dfy"
+include "MerkleTrees.dfy"
+include "NextPathInCompleteTreesLemmas.dfy"
+include "PathInCompleteTrees.dfy"
+include "SeqOfBits.dfy"
+include "Trees2.dfy"
+
+/**
+ *  Imperative version of algorithm.
+ */
+module IncAlgoV5 {
+ 
+    import opened DiffTree
+    import opened IncAlgoV3
+    import opened CompleteTrees
+    import opened ComputeRootPath
+    import opened GenericComputation
+    import opened Helpers
+    import opened MerkleTrees
+    import opened NextPathInCompleteTreesLemmas
+    import opened PathInCompleteTrees
+    import opened SeqOfBits
+    import opened Trees
+
+    /**
+     *  @todo: division by power2 computation is assumed. Prove it.
+     */
+    method merkleV1(h : nat, k : nat, valOnLeftAt : seq<int>, seed: int) 
+                                                        returns (r : int, next: seq<int>)
+        requires 1 <= h == |valOnLeftAt|
+        requires k < power2(h)
+
+        // ensures (r, next) == computeRootPathDiffAndLeftSiblingsUpv4(h, k, valOnLeftAt, seed)
+        // ensures r == computeRootPathDiffAndLeftSiblingsUpv4(h, k, valOnLeftAt, seed).0
+    {
+        var i := 0;
+        var k' := k;
+        
+        // divIsZero(k, power2(h));
+        // assert(k / power2(h) == 0);
+        // assert(k' == k / power2(h - i));
+        r := seed ;
+        next := [] ; 
+
+        ghost var h1 := h;
+
+        //  initial computation
+        assert(h - i == |valOnLeftAt|);
+        assert(h1 == h - i);
+        assert(k' < power2(h - i));
+       
+        //  compute result with computeRootPathDiffAndLeftSiblingsUpv4c
+        ghost var (r', next') := computeRootPathDiffAndLeftSiblingsUpv4c(h, k, valOnLeftAt, seed, []);
+
+        //  need this fact to probve next assert
+        assert(valOnLeftAt == valOnLeftAt[..h - i]);
+        assert(k' < power2(h1));
+        assert(h1 == h);
+        assert(
+            (r', next') ==   computeRootPathDiffAndLeftSiblingsUpv4c(h1, k', valOnLeftAt[..h1], r, next)
+        );
+
+        while (i < h)
+
+            invariant 0 <= i <= h
+            invariant i == |valOnLeftAt[.. i]|
+            // invariant i > 0 ==> 0 <= k' < power2(h1) 
+            invariant 0 <= k' < power2(h1)
+            invariant h1 == h - i
+            // invariant k' == k / power2(h - i)      //  Inv4
+
+            invariant (r', next') == computeRootPathDiffAndLeftSiblingsUpv4c(h1, k', valOnLeftAt[..h1], r, next);
+
+
+            decreases h - i 
+        {
+            if k' % 2 == 0 {
+                next := [r] + next ;
+                r := diff(r, 0);
+                assert(
+                    (r', next')
+                    ==
+                    computeRootPathDiffAndLeftSiblingsUpv4c(h1 - 1, k' / 2,
+                            valOnLeftAt[..h1][.. h1 - 1], r, next)
+                );
+            } else {
+                next := [valOnLeftAt[h - i - 1]] + next ;
+                r := diff(valOnLeftAt[h - i - 1], r);
+                assert(
+                    (r', next')
+                    ==
+                    computeRootPathDiffAndLeftSiblingsUpv4c(
+                            h1 - 1,
+                            k' / 2,
+                            valOnLeftAt[..h1][.. h1 - 1],   
+                             r,
+                            next)
+                );
+            }
+            //  the following is used to prove Inv4
+            assume(k / power2(h - i)) / 2 == k / (power2(h - i) / 2);
+            assert(valOnLeftAt[..h1 - 1] == valOnLeftAt[..h1][..h1 - 1]);
+            i := i + 1;
+            k' := k' / 2;
+            h1 := h1 - 1;
+            assert(
+                (r', next') == 
+                computeRootPathDiffAndLeftSiblingsUpv4c(h1, k', valOnLeftAt[..h1], r, next)
+            );
+            
+        }
+        //  after the loop we get the result
+        assert(
+            (r', next') == 
+                computeRootPathDiffAndLeftSiblingsUpv4c(h1, k', valOnLeftAt[..h1], r, next)
+        );
+        //  and because h1 is 0 
+        assert(
+            (r', next') == 
+                computeRootPathDiffAndLeftSiblingsUpv4c(0, k', valOnLeftAt[..h1], r', next')
+        );
+        assert(
+            (r, next) == (r', next')
+            ==
+            computeRootPathDiffAndLeftSiblingsUpv4c(h, k, valOnLeftAt, seed, [])
+        );
+    }
+
+    lemma divIsZero(n : nat, m : nat) 
+        requires n < m
+        ensures n / m == 0 
+    {
+
+    }
+ }
